@@ -1,0 +1,13 @@
+module
+
+public import Roolean.QfBv.Checker
+
+public def solve {v: VarWidths} (α) [Domain α] [AbstractDomain α]
+  (term: BvTerm v 1) : Option Bool := do
+  -- brute-force by splitting everything
+  let splitTree: Proof.Node v := Fin.foldl v.size (λ (splitTree: Proof.Node v) varIndex =>
+    Fin.foldl (v.varWidth varIndex) (λ splitTree bitIndex =>
+        Proof.Node.Split varIndex bitIndex splitTree splitTree) splitTree
+    ) Proof.Node.Relevant
+
+  computeSat α term splitTree
